src/Finish/IEF.v
@@ -1,29 +1,24 @@
 Require Import HJ.Finish.Lang.
 Require Import HJ.Vars.
-Require Import Aniceto.Graphs.Bipartite.Bipartite.
-Require Import Aniceto.Graphs.Graph.
 
 
 Import FinishNotations.
 Local Open Scope finish_scope.
 
 Inductive IEF (t:tid) (f:finish) : Prop :=
-  enclosing_def:
-    (forall c, Sub c f -> ~ Registered t c) ->
+  ief_def:
+    (forall c, Sub c f -> ~ In t c) ->
     Registered t f ->
     IEF t f.
 
-Inductive FIDPath (f:finish) : finish -> fid -> Prop :=
+(**
+  [FIDPath f1 l f2] means that we can go from [f1] to [f2] according to path [l].
+ *)
+Inductive FIDPath (f:finish) : fid -> finish -> Prop :=
   | fid_path_nil:
-     FIDPath f f nil
-   | fid_path_cons:
-     forall t' f' l f'',
-     FIDPath f f' l ->
-     Child (t' <| f') f'' ->
-     FIDPath f f'' (t'::l) % list.
-
-Inductive FID (f:finish) (i:fid) : Prop :=
-  fid_def:
-    forall f',
-    FIDPath f' f i ->
-    FID f i.
+     FIDPath f nil f
+  | fid_path_cons:
+    forall t' f' l f'',
+    FIDPath f l f' ->
+    Child (t' <| f') f'' ->
+    FIDPath f (t'::l) % list f''.
